coq code refactoring

Common.v
@@ -8,20 +8,67 @@ Open Scope list_scope.
 Definition admit {T: Type} : T. Admitted.
 
 Module Procedure.
-  Definition id := nat.
+
+Definition id := nat.
+
 End Procedure.
 
 Module Component.
-  Definition id := nat.
 
-  Record interface :=
-    mkCompInterface {
-        name : id;
-        export : nat;
-        import : list (id * Procedure.id)
-    }.
+Definition id := nat.
+
+Record interface := mkCompInterface {
+  name : id;
+  export : nat;
+  import : list (id * Procedure.id)
+}.
+
 End Component.
 
 Module Program.
-  Definition interface := list (option Component.interface).
+
+Definition interface := list Component.interface.
+
 End Program.
+
+Module Util.
+
+Fixpoint mem x xs :=
+  match xs with
+  | [] => false
+  | x' :: xs' => if x =? x' then true else mem x xs'
+  end.
+
+Lemma not_in_implies_mem_false :
+  forall x xs,
+    ~ (In x xs) -> mem x xs = false.
+Proof.
+  intros.
+  induction xs.
+  - reflexivity.
+  - simpl.
+    apply not_in_cons in H. destruct H.
+    unfold not in H.
+    destruct (x =? a) eqn:Heq_xa.
+    + exfalso. apply beq_nat_true in Heq_xa.
+      apply H. apply Heq_xa.
+    + apply IHxs. apply H0.
+Qed.
+
+Lemma in_implies_mem_true :
+  forall x xs,
+    In x xs -> mem x xs = true.
+Proof.
+  intros.
+  induction xs.
+  - exfalso. apply (in_nil H).
+  - simpl.
+    destruct (x =? a) eqn:Heq_xa.
+    + reflexivity.
+    + apply IHxs. apply in_inv in H. destruct H.
+      * exfalso. rewrite beq_nat_false_iff in Heq_xa.
+        apply Heq_xa. symmetry. apply H.
+      * apply H.
+Qed.
+
+End Util.
