LTT.v
@@ -11,6 +11,20 @@ Definition stack:= list (Component.id * Memory.address).
 Definition state : Type := 
   (Component.id * stack * Memory.data * Register.data * Memory.address).
 
+Record global_env := mkGlobalEnv {
+  get_interfaces : Program.interface;
+  get_entrypoints : EntryPoint.data;
+}.
+
+Record global_env_wf (G : global_env) := mkGlobalEnvWF {
+  entrypoints_exist :
+    forall CI C,
+      In CI (get_interfaces G) ->
+      Component.name CI = C ->
+      M.In C (get_entrypoints G) /\
+      exists addrs, M.MapsTo C addrs (get_entrypoints G);
+}.
+
 Definition eval_binop (e : binop) (a b : nat) : nat :=
   match e with
   | Add   => a + b
@@ -20,92 +34,92 @@ Definition eval_binop (e : binop) (a b : nat) : nat :=
   | Leq   => if a <=? b then 1 else 0
   end.
 
-Reserved Notation "Is ; E |-LTT s1 '=>[' t ']' s2" (at level 40).
+Reserved Notation "G |-LTT s1 '=>[' t ']' s2" (at level 40).
 
-Inductive step (Is : Program.interface) (E : EntryPoint.data)
+Inductive step (G : global_env)
   : state -> trace -> state -> Prop :=
+| Nop: forall mem C pc d regs,
+    executing Nop C mem pc ->
+    G |-LTT (C,d,mem,regs,pc) =>[E0] (C,d,mem,regs,pc+1)
 
-  | Nop: forall mem C pc d regs,
-      executing Nop C mem pc ->
-      Is;E |-LTT (C,d,mem,regs,pc) =>[E0] (C,d,mem,regs,pc+1)
+| Const: forall mem C pc r cval d regs regs',
+    executing (Const cval r) C mem pc ->
+    regs' = Register.set r cval regs ->
+    G |-LTT (C,d,mem,regs,pc) =>[E0] (C,d,mem,regs',pc+1)
 
-  | Const: forall mem C pc r cval d regs regs',
-      executing (Const cval r) C mem pc ->
-      regs' = Register.set r cval regs ->
-      Is;E |-LTT (C,d,mem,regs,pc) =>[E0] (C,d,mem,regs',pc+1)
+| Mov: forall mem C pc r1 r2 regs regs' d,
+    executing (Mov r1 r2) C mem pc ->
+    regs' = Register.set r2 (Register.get r1 regs) regs ->
+    G |-LTT (C,d,mem,regs,pc) =>[E0] (C,d,mem,regs',pc+1)
 
-  | Mov: forall mem C pc r1 r2 regs regs' d,
-      executing (Mov r1 r2) C mem pc ->
-      regs' = Register.set r2 (Register.get r1 regs) regs ->
-      Is;E |-LTT (C,d,mem,regs,pc) =>[E0] (C,d,mem,regs',pc+1)
+| BinOp: forall mem C pc r1 r1val r2 r2val r3 regs regs' d op,
+    executing (BinOp op r1 r2 r3) C mem pc ->
+    r1val = Register.get r1 regs ->
+    r2val = Register.get r2 regs ->
+    regs' = Register.set r3 (eval_binop op r1val r2val) regs ->
+    G |-LTT (C,d,mem,regs,pc) =>[E0] (C,d,mem,regs',pc+1)
 
-  | BinOp: forall mem C pc r1 r1val r2 r2val r3 regs regs' d op,
-      executing (BinOp op r1 r2 r3) C mem pc ->
-      r1val = Register.get r1 regs ->
-      r2val = Register.get r2 regs ->
-      regs' = Register.set r3 (eval_binop op r1val r2val) regs ->
-      Is;E |-LTT (C,d,mem,regs,pc) =>[E0] (C,d,mem,regs',pc+1)
+| Load: forall mem C pc r1 r2 regs regs' d addr memval,
+    executing (Load r1 r2) C mem pc ->
+    addr = Register.get r1 regs ->
+    Some memval = Memory.get mem C addr ->
+    regs' = Register.set r2 memval regs ->
+    G |-LTT (C,d,mem,regs,pc) =>[E0] (C,d,mem,regs',pc+1)
 
-  | Load: forall mem C pc r1 r2 regs regs' d addr memval,
-      executing (Load r1 r2) C mem pc ->
-      addr = Register.get r1 regs ->
-      Some memval = Memory.get mem C addr ->
-      regs' = Register.set r2 memval regs ->
-      Is;E |-LTT (C,d,mem,regs,pc) =>[E0] (C,d,mem,regs',pc+1)
+| Store: forall mem C pc r1 r2 regs d addr value mem',
+    executing (Store r1 r2) C mem pc->
+    addr = Register.get r1 regs ->
+    value = Register.get r2 regs ->
+    mem' = Memory.set mem C addr value ->
+    G |-LTT (C,d,mem,regs,pc) =>[E0] (C,d,mem',regs,pc+1)
 
-  | Store: forall mem C pc r1 r2 regs d addr value mem',
-      executing (Store r1 r2) C mem pc->
-      addr = Register.get r1 regs ->
-      value = Register.get r2 regs ->
-      mem' = Memory.set mem C addr value ->
-      Is;E |-LTT (C,d,mem,regs,pc) =>[E0] (C,d,mem',regs,pc+1)
+| Jal: forall mem C pc val r regs regs' d,
+    executing (Jal r) C mem pc->
+    val = Register.get r regs ->
+    regs' = Register.set r (pc+1) regs ->
+    G |-LTT (C,d,mem,regs,pc) =>[E0] (C,d,mem,regs',val)
 
-  | Jal: forall mem C pc val r regs regs' d,
-      executing (Jal r) C mem pc->
-      val = Register.get r regs ->
-      regs' = Register.set r (pc+1) regs ->
-      Is;E |-LTT (C,d,mem,regs,pc) =>[E0] (C,d,mem,regs',val)
+| Jump: forall mem C pc addr r regs d,
+    executing (Jump r) C mem pc->
+    Register.get r regs = addr ->
+    G |-LTT (C,d,mem,regs,pc) =>[E0] (C,d,mem,regs,addr)
 
-  | Jump: forall mem C pc addr r regs d,
-      executing (Jump r) C mem pc->
-      Register.get r regs = addr ->
-      Is;E |-LTT (C,d,mem,regs,pc) =>[E0] (C,d,mem,regs,addr)
+| BnzNZ: forall mem C pc offset r regs d,
+    executing (Bnz r offset) C mem pc ->
+    Register.get r regs <> 0 ->
+    G |-LTT (C,d,mem,regs,pc) =>[E0] (C,d,mem,regs,pc+offset)
 
-  | BnzNZ: forall mem C pc offset r regs d,
-      executing (Bnz r offset) C mem pc ->
-      Register.get r regs <> 0 ->
-      Is;E |-LTT (C,d,mem,regs,pc) =>[E0] (C,d,mem,regs,pc+offset)
+| BnzZ: forall mem C pc offset r regs d,
+    executing (Bnz r offset) C mem pc ->
+    Register.get r regs = 0 ->
+    G |-LTT (C,d,mem,regs,pc) =>[E0] (C,d,mem,regs,pc+1)
 
-  | BnzZ: forall mem C pc offset r regs d,
-      executing (Bnz r offset) C mem pc ->
-      Register.get r regs = 0 ->
-      Is;E |-LTT (C,d,mem,regs,pc) =>[E0] (C,d,mem,regs,pc+1)
+| Call: forall mem C pc regs d d' C' P,
+    executing (Call C' P) C mem pc ->
+    call_is_public_and_exists (get_interfaces G) C' P ->
+    call_is_in_imports (get_interfaces G) C C' P ->
+    C' <> C ->
+    d' = (C,pc+1) :: d ->
+    let t := [ECall C P (Register.get Register.R_COM regs) C'] in
+    let E := get_entrypoints G in
+    G |-LTT (C,d,mem,regs,pc) =>[t]
+            (C',d',mem,regs,EntryPoint.get C' P E)
 
-  | Call: forall mem C pc regs d d' C' P,
-      executing (Call C' P) C mem pc ->
-      call_exists Is C' P ->
-      call_permitted Is C C' P ->
-      C' <> C ->
-      d' = (C,pc+1) :: d ->
-      let t := [ECall C P (Register.get Register.R_COM regs) C'] in
-      Is;E |-LTT (C,d,mem,regs,pc) =>[t]
-                 (C',d',mem,regs,EntryPoint.get C' P E)
+| Return: forall mem C pc pc' d' regs d C',
+    executing Return C mem pc ->
+    d = (C',pc') :: d' ->
+    C <> C' ->
+    let t := [ERet C (Register.get Register.R_COM regs) C'] in
+    G |-LTT (C,d,mem,regs,pc) =>[t] (C',d',mem,regs,pc')
 
-  | Return: forall mem C pc pc' d' regs d C',
-      executing Return C mem pc ->
-      d = (C',pc') :: d' ->
-      C <> C' ->
-      let t := [ERet C (Register.get Register.R_COM regs) C'] in
-      Is;E |-LTT (C,d,mem,regs,pc) =>[t] (C',d',mem,regs,pc')
-
-  where "Is ; E |-LTT s1 '=>[' t ']' s2" := (step Is E s1 t s2).
+where "G |-LTT s1 '=>[' t ']' s2" := (step G s1 t s2).
 
 Lemma epsilon_step_preserves_component_and_stack:
-  forall Is E C d mem regs pc C' d' mem' regs' pc',
-    Is; E |-LTT (C,d,mem,regs,pc) =>[E0] (C',d',mem',regs',pc') ->
+  forall G C d mem regs pc C' d' mem' regs' pc',
+    G |-LTT (C,d,mem,regs,pc) =>[E0] (C',d',mem',regs',pc') ->
     C' = C /\ d' = d.
 Proof.
-  intros Is E C d mem regs pc C' d' mem' regs' pc' Hstep.
+  intros G C d mem regs pc C' d' mem' regs' pc' Hstep.
   inversion Hstep; subst;
     split; trivial.
 Qed.
@@ -114,12 +128,12 @@ Lemma epsilon_step_weakening:
   forall Is E C d1 mem mem' cmem cmem' regs regs' pc pc',
     M.MapsTo C cmem  mem ->
     M.MapsTo C cmem' mem' ->
-    Is; E |-LTT (C,d1,mem,regs,pc) =>[E0] (C,d1,mem',regs',pc') ->
+    (mkGlobalEnv Is E) |-LTT (C,d1,mem,regs,pc) =>[E0] (C,d1,mem',regs',pc') ->
   forall E' d2 wmem,
     M.MapsTo C cmem wmem ->
     exists wmem',
       M.MapsTo C cmem' wmem' ->
-      Is; E' |-LTT (C,d2,wmem,regs,pc) =>[E0] (C,d2,wmem',regs',pc').
+      (mkGlobalEnv Is E') |-LTT (C,d2,wmem,regs,pc) =>[E0] (C,d2,wmem',regs',pc').
 Proof.
   intros Is E C d1 mem mem' cmem cmem' regs regs' pc pc'.
   intros HCmem HCmem' Hstep.
@@ -197,37 +211,37 @@ Proof.
 Qed.
 
 Theorem LTT_determinism :
-  forall Is E s t s1 s2,
-    Is;E |-LTT s =>[t] s1 ->
-    Is;E |-LTT s =>[t] s2 ->
+  forall G s t s1 s2,
+    G |-LTT s =>[t] s1 ->
+    G |-LTT s =>[t] s2 ->
     s1 = s2.
 Proof.
-  intros Is E s t s1 s2 E1 E2.
-  inversion E1 as [ mem C pc d regs Hexec |
-                    mem C pc d regs w0 w1 w2 Hexec |
-                    mem C pc d regs w0 w1 w2 Hexec |
-                    mem C pc d regs w0 w1 w2 w3 w4 w5 w6 Hexec |
-                    mem C pc d regs w0 w1 w2 w3 w4 Hexec |
-                    mem C pc d regs w0 w1 w2 w3 w4 Hexec |
-                    mem C pc d regs w0 w1 w2 Hexec |
-                    mem C pc d regs w0 w1 Hexec |
-                    mem C pc d regs w0 w1 Hexec |
-                    mem C pc d regs w0 w1 Hexec |
-                    mem C pc d regs w0 w1 w2 Hexec |
-                    mem C pc d regs w0 w1 w2 Hexec ];
+  intros G s t s1 s2 E1 E2.
+  inversion E1 as [ ? ? ? ? ? Hexec |
+                    ? ? ? ? ? ? ? ? Hexec |
+                    ? ? ? ? ? ? ? ? Hexec |
+                    ? ? ? ? ? ? ? ? ? ? ? ? Hexec |
+                    ? ? ? ? ? ? ? ? ? ? Hexec |
+                    ? ? ? ? ? ? ? ? ? ? Hexec |
+                    ? ? ? ? ? ? ? ? Hexec |
+                    ? ? ? ? ? ? ? Hexec |
+                    ? ? ? ? ? ? ? Hexec |
+                    ? ? ? ? ? ? ? Hexec |
+                    ? ? ? ? ? ? ? ? Hexec |
+                    ? ? ? ? ? ? ? ? Hexec ];
     subst;
-    inversion E2 as [ mem'' C'' pc'' d'' regs'' Hexec' |
-                      mem'' C'' pc'' d'' regs'' z0 z1 z2 Hexec' |
-                      mem'' C'' pc'' d'' regs'' z0 z1 z2 Hexec' |
-                      mem'' C'' pc'' d'' regs'' z0 z1 z2 z3 z4 z5 z6 Hexec' |
-                      mem'' C'' pc'' d'' regs'' z0 z1 z2 z3 z4 Hexec' |
-                      mem'' C'' pc'' d'' regs'' z0 z1 z2 z3 z4 Hexec' |
-                      mem'' C'' pc'' d'' regs'' z0 z1 z2 Hexec' |
-                      mem'' C'' pc'' d'' regs'' z0 z1 Hexec' |
-                      mem'' C'' pc'' d'' regs'' z0 z1 Hexec' |
-                      mem'' C'' pc'' d'' regs'' z0 z1 Hexec' |
-                      mem'' C'' pc'' d'' regs'' z0 z1 z2 Hexec' |
-                      mem'' C'' pc'' d'' regs'' z0 z1 z2 Hexec' ];
+      inversion E2 as [ ? ? ? ? ? Hexec' |
+                        ? ? ? ? ? ? ? ? Hexec' |
+                        ? ? ? ? ? ? ? ? Hexec' |
+                        ? ? ? ? ? ? ? ? ? ? ? ? Hexec' |
+                        ? ? ? ? ? ? ? ? ? ? Hexec' |
+                        ? ? ? ? ? ? ? ? ? ? Hexec' |
+                        ? ? ? ? ? ? ? ? Hexec' |
+                        ? ? ? ? ? ? ? Hexec' |
+                        ? ? ? ? ? ? ? Hexec' |
+                        ? ? ? ? ? ? ? Hexec' |
+                        ? ? ? ? ? ? ? ? Hexec' |
+                        ? ? ? ? ? ? ? ? Hexec' ];
     subst;
     (* same step *)
     try reflexivity;
