Machine.v
@@ -6,152 +6,179 @@ Require Import Coq.Structures.OrdersEx.
 Require Import Coq.Structures.OrdersAlt.
 
 Module AbstractMachine.
-  Module backNat_as_OT := Backport_OT Nat_as_OT.
-  Module M := FMapAVL.Make backNat_as_OT.
-  Module P := WProperties_fun Nat_as_OT M.
-  Module F := P.F.
 
-  Module Register.
-    Definition data : Type := M.t nat.
+Module backNat_as_OT := Backport_OT Nat_as_OT.
+Module M := FMapAVL.Make backNat_as_OT.
+Module P := WProperties_fun Nat_as_OT M.
+Module F := P.F.
 
-    Inductive reg : Set :=
-      R_PC | R_ONE | R_COM | R_AUX1 | R_AUX2 | R_RA | R_SP.
+Module Register.
+  Definition data : Type := M.t nat.
 
-    Definition to_nat (r : reg) : nat :=
-      match r with
-      | R_PC   => 0
-      | R_ONE  => 1
-      | R_COM  => 2
-      | R_AUX1 => 3
-      | R_AUX2 => 4
-      | R_RA   => 5
-      | R_SP   => 6
-      end.
+  Inductive reg : Set :=
+    R_PC | R_ONE | R_COM | R_AUX1 | R_AUX2 | R_RA | R_SP.
 
-    Definition get (r : reg) (regs : data) : nat :=
-      match M.find (to_nat r) regs with 
-      | Some val => val
-      (* this should never happen (i.e. regs should be well-formed) *)
-      | None => 0
-      end.
+  Definition to_nat (r : reg) : nat :=
+    match r with
+    | R_PC   => 0
+    | R_ONE  => 1
+    | R_COM  => 2
+    | R_AUX1 => 3
+    | R_AUX2 => 4
+    | R_RA   => 5
+    | R_SP   => 6
+    end.
 
-    Definition set (r : reg) (val : nat) (regs : data) : data :=
-      M.add (to_nat r) val regs.
-  End Register.
+  Definition get (r : reg) (regs : data) : nat :=
+    match M.find (to_nat r) regs with
+    | Some val => val
+    (* this should never happen (i.e. regs should be well-formed) *)
+    | None => 0
+    end.
 
-  Module Memory.
-    Definition address := nat.
-    Definition data: Type := M.t (list nat).
+  Definition set (r : reg) (val : nat) (regs : data) : data :=
+    M.add (to_nat r) val regs.
+End Register.
 
-    Definition get mem C a : option nat :=
-      match M.find C mem with
-      | Some cmem => Some (nth a cmem 0)
-      | None => None
-      end.
+Module Memory.
+  Definition address := nat.
+  Definition data: Type := M.t (list nat).
 
-    Fixpoint local_update (a : address) (val : nat) (lmem : list nat) :=
-      match lmem with
-      | [] => [] 
-      | h::t =>
-        match a with
-        | 0 => val :: t
-        | S a' => h :: local_update a' val t
-        end
-      end.
+  Definition get mem C a : option nat :=
+    match M.find C mem with
+    (* when the address 'a' points outside of memory, we just return 0 *)
+    | Some cmem => Some (nth a cmem 0)
+    | None => None
+    end.
 
-    Definition set mem C a val :=
-      match M.find C mem with
-      | Some cmem =>
-        M.add C (local_update a val cmem) mem
-      | None => mem
-      end.
+  Fixpoint local_update (a : address) (val : nat) (lmem : list nat) :=
+    match lmem with
+    | [] =>
+      (* extend the memory, since the address points outside of it *)
+      (* (we are modeling an infinite memory, hence this extension) *)
+      match a with
+      | 0 => [val]
+      | S a' => 0 :: local_update a' val []
+      end
+    | val' :: lmem' =>
+      match a with
+      | 0 => val :: lmem'
+      | S a' => val' :: local_update a' val lmem'
+      end
+    end.
 
-    Definition of_component C mem : option (list nat) := M.find C mem.
+  Definition set mem C a val :=
+    match M.find C mem with
+    | Some cmem =>
+      M.add C (local_update a val cmem) mem
+    | None => mem
+    end.
 
-    Definition inject C cmem (mem : data) := M.add C cmem mem.
+  Definition of_component C mem : option (list nat) := M.find C mem.
 
-    Definition filter (pc : list Component.id) (mem : data) :=
-      P.filter (fun C _ => existsb (fun C' => C =? C') pc) mem.
+  Definition inject C cmem (mem : data) := M.add C cmem mem.
 
-    Definition singleton C cmem : data :=
-      M.add C cmem (M.empty (list Memory.address)).
+  Definition filter (pc : list Component.id) (mem : data) :=
+    P.filter (fun C _ => existsb (fun C' => C =? C') pc) mem.
 
-    Lemma get_works_locally :
-      forall mem cmem C i,
-        of_component C mem = Some cmem ->
-        get mem C i = get (singleton C cmem) C i.
-    Proof.
-      intros.
-      unfold singleton, get.
-      unfold of_component in H.
-      rewrite H. rewrite F.add_eq_o; reflexivity.
-    Qed.
-  End Memory.
+  Definition singleton C cmem : data :=
+    M.add C cmem (M.empty (list Memory.address)).
+
+  Lemma get_works_locally :
+    forall mem cmem C i,
+      of_component C mem = Some cmem ->
+      get mem C i = get (singleton C cmem) C i.
+  Proof.
+    intros.
+    unfold singleton, get.
+    unfold of_component in H.
+    rewrite H. rewrite F.add_eq_o; reflexivity.
+  Qed.
+End Memory.
  
-  Inductive binop :=
-    Add | Minus | Mul | Eq | Leq.
+Inductive binop := Add | Minus | Mul | Eq | Leq.
 
-  Inductive instr :=
-    | Nop    : instr
-    (* register operations *)
-    | Const  : nat -> Register.reg -> instr
-    | Mov    : Register.reg -> Register.reg -> instr
-    | BinOp  : binop -> Register.reg -> Register.reg -> Register.reg -> instr
-    (* memory operations *)
-    | Load   : Register.reg -> Register.reg -> instr
-    | Store  : Register.reg -> Register.reg -> instr
-    (* conditional and unconditional jumps *)
-    | Bnz    : Register.reg -> nat -> instr
-    | Jump   : Register.reg -> instr
-    | Jal    : Register.reg -> instr
-    (* components interaction *) 
-    | Call   : Component.id -> Procedure.id -> instr
-    | Return : instr
-    (* termination *)
-    | Halt   : instr.
+Inductive instr :=
+| Nop    : instr
+(* register operations *)
+| Const  : nat -> Register.reg -> instr
+| Mov    : Register.reg -> Register.reg -> instr
+| BinOp  : binop -> Register.reg -> Register.reg -> Register.reg -> instr
+(* memory operations *)
+| Load   : Register.reg -> Register.reg -> instr
+| Store  : Register.reg -> Register.reg -> instr
+(* conditional and unconditional jumps *)
+| Bnz    : Register.reg -> nat -> instr
+| Jump   : Register.reg -> instr
+| Jal    : Register.reg -> instr
+(* components interaction *)
+| Call   : Component.id -> Procedure.id -> instr
+| Return : instr
+(* termination *)
+| Halt   : instr.
 
-  Module EncDec.
-    Definition decode (n : option nat) : option instr := admit.
-    Definition encode (i:instr) : option nat := admit.
+Module EncDec.
+  (* we assume to have a decoder for our instruction. Later we could try
+     to think of a simple representation for instructions and implement
+     it for real *)
 
-    Theorem decode_encode : forall i, decode (encode i) = Some i.
-    Proof. Admitted.
-  End EncDec.
+  Definition decode (n : option nat) : option instr := admit.
+  Definition encode (i:instr) : option nat := admit.
 
-  Module EntryPoint.
-    Definition data : Type := M.t (list Memory.address).
+  Theorem decode_encode : forall i, decode (encode i) = Some i.
+  Proof. Admitted.
+End EncDec.
 
-    Definition get C P E : Memory.address :=
-      match M.find C E with
-      | Some E' => nth P E' 0 
-      | None => 0
-      end.
+Module EntryPoint.
+  Definition data : Type := M.t (list Memory.address).
 
-    Definition mem C (E : data) : bool := M.mem C E.
+  Definition get C P E : Memory.address :=
+    match M.find C E with
+    | Some E' => nth P E' 0
+    | None => 0
+    end.
 
-    Definition of_component C E : option (list Memory.address) :=
-      M.find C E.
+  Definition mem C (E : data) : bool := M.mem C E.
 
-    Definition singleton C E : data := M.add C E (M.empty _).
+  Definition of_component C E : option (list Memory.address) :=
+    M.find C E.
 
-    Definition filter (pc : list Component.id) (E : data) :=
-      P.filter (fun C _ => existsb (fun C' => C =? C') pc) E.
-  End EntryPoint.
+  Definition singleton C E : data := M.add C E (M.empty _).
 
-  Definition call_exists
-             (Is : Program.interface)
-             (C : Component.id) (P : Procedure.id) :=
-    forall comp_interface,
-      nth C Is None = Some comp_interface ->
-      C < Component.export comp_interface.
+  Definition filter (pc : list Component.id) (E : data) :=
+    P.filter (fun C _ => existsb (fun C' => C =? C') pc) E.
 
-  Definition call_permitted
-             (Is : Program.interface)
-             (C C': Component.id) (P : Procedure.id) :=
-    forall comp_interface,
-      nth C Is None = Some comp_interface ->
-      In (C',P) (Component.import comp_interface).
+  Lemma get_works_locally :
+    forall E E' C P addrs,
+      M.MapsTo C addrs E ->
+      M.MapsTo C addrs E' ->
+      get C P E = get C P E'.
+  Proof.
+    intros E E' C P addrs HEaddrs HE'addrs.
+    unfold get.
+    rewrite F.find_mapsto_iff in HEaddrs, HE'addrs.
+    rewrite <- HEaddrs in HE'addrs.
+    inversion HE'addrs as [HEeqE'].
+    rewrite HEeqE'.
+    reflexivity.
+  Qed.
+End EntryPoint.
 
-  Definition executing i C mem pc :=
-    EncDec.decode (Memory.get mem C pc) = Some i.
+Definition call_is_public_and_exists
+           (Is : Program.interface)
+           (C : Component.id) (P : Procedure.id) :=
+  forall CI,
+    find (fun C' => C =? Component.name C') Is = Some CI ->
+    C < Component.export CI.
+
+Definition call_is_in_imports
+           (Is : Program.interface)
+           (C C': Component.id) (P : Procedure.id) :=
+  forall CI,
+    find (fun C' => C =? Component.name C') Is = Some CI ->
+    In (C',P) (Component.import CI).
+
+Definition executing i C mem pc :=
+  EncDec.decode (Memory.get mem C pc) = Some i.
+
 End AbstractMachine.
