PLTT.v
@@ -4,148 +4,162 @@ Require Import Traces.
 Require Import LTT.
 
 Module PLTT.
-  Include AbstractMachine.
 
-  Definition stack := list (Component.id * option Memory.address).
+Include AbstractMachine.
 
-  Definition program_state : Type :=
-    (Component.id * stack * Memory.data * Register.data * Memory.address).
-  Definition context_state : Type :=
-    (Component.id * stack * Memory.data).
+Definition stack := list (Component.id * option Memory.address).
 
-  Inductive partial_state : Type :=
-    | PC : program_state -> partial_state
-    | CC : context_state -> partial_state.
+Definition program_state : Type :=
+  (Component.id * stack * Memory.data * Register.data * Memory.address).
+Definition context_state : Type :=
+  (Component.id * stack * Memory.data).
 
-  Fixpoint to_partial_stack (s : LTT.stack) (pc : list Component.id)
-    : PLTT.stack :=
-    match s with
-    | [] => []
-    | (C,i) :: s' =>
-      if existsb (fun C' => C =? C') pc then
-        (C,Some i) :: to_partial_stack s' pc
-      else
-        (C,None) :: to_partial_stack s' pc
-    end.
+Inductive partial_state : Type :=
+  | PC : program_state -> partial_state
+  | CC : context_state -> partial_state.
 
-  Lemma push_by_prog_preserves_partial_stack :
-    forall s ps pc C i,
-      existsb (fun C' => C =? C') pc = true ->
-      to_partial_stack s pc = ps ->
-      to_partial_stack ((C,i)::s) pc = (C,Some i) :: ps.
-  Proof.
-    intros s ps pc C i Hprogturn H.
-    simpl. rewrite Hprogturn. rewrite H. reflexivity.
-  Qed.
+Definition to_partial_frame pc frame : Component.id * option Memory.address :=
+  match frame with (C,i) =>
+    if Util.mem C pc then (C, Some i) else (C, None)
+  end.
 
-  Lemma push_by_context_preserves_partial_stack :
-    forall s ps pc C i,
-      existsb (fun C' => C =? C') pc = false ->
-      to_partial_stack s pc = ps ->
-      to_partial_stack ((C,i)::s) pc = (C,None) :: ps.
-  Proof.
-    intros s ps pc C i Hprogturn H.
-    simpl. rewrite Hprogturn. rewrite H. reflexivity.
-  Qed.
+Definition to_partial_stack (s : LTT.stack) (pc : list Component.id) :=
+  map (to_partial_frame pc) s.
 
-  Definition is_program_component
-             (C : Component.id)
-             (E : EntryPoint.data) : Prop :=
-    EntryPoint.mem C E = true.
+Lemma push_by_prog_preserves_partial_stack :
+  forall s ps pc C i,
+    Util.mem C pc = true ->
+    to_partial_stack s pc = ps ->
+    to_partial_stack ((C,i)::s) pc = (C,Some i) :: ps.
+Proof.
+  intros s ps pc C i Hprogturn H.
+  simpl. rewrite Hprogturn. rewrite H. reflexivity.
+Qed.
 
-  Definition is_context_component
-             (C : Component.id)
-             (E : EntryPoint.data) : Prop :=
-    EntryPoint.mem C E = false.
+Lemma push_by_context_preserves_partial_stack :
+  forall s ps pc C i,
+    ~ (In C pc) ->
+    to_partial_stack s pc = ps ->
+    to_partial_stack ((C,i)::s) pc = (C,None) :: ps.
+Proof.
+  intros s ps pc C i Hprogturn Hpstack.
+  simpl. apply Util.not_in_implies_mem_false in Hprogturn.
+  rewrite Hprogturn. rewrite Hpstack. reflexivity.
+Qed.
 
-  Reserved Notation "Is ; E |-PLTT s1 '=>[' t ']' s2" (at level 40).
+Record global_env := mkGlobalEnv {
+  get_interfaces : Program.interface;
+  get_entrypoints : EntryPoint.data;
+  get_split : list Component.id
+}.
 
-  Inductive step (Is : Program.interface) (E : EntryPoint.data)
-    : partial_state -> trace -> partial_state -> Prop :=
+Record global_env_wf (G : global_env) := mkGlobalEnvWF {
+  entrypoints_exist :
+    forall CI C,
+      In CI (get_interfaces G) ->
+      Component.name CI = C ->
+      M.In C (get_entrypoints G) /\
+      exists addrs, M.MapsTo C addrs (get_entrypoints G);
+  split_wellformed :
+    forall C,
+      In C (get_split G) ->
+      exists CI, In CI (get_interfaces G) /\ Component.name CI = C
+}.
 
-    | Program_Epsilon:
-        forall C s ps mem mem' wmem wmem' cmem cmem' regs regs' pc pc',
-          M.MapsTo C cmem wmem ->
-          M.MapsTo C cmem' wmem' ->
-          LTT.step Is E (C,s,wmem,regs,pc) E0 (C,s,wmem',regs',pc') ->
-          M.MapsTo C cmem mem ->
-          M.MapsTo C cmem' mem' ->
-          Is;E |-PLTT (PC (C,ps,mem,regs,pc)) =>[E0] (PC (C,ps,mem',regs',pc'))
+Definition is_program_component C (prog_comps : list Component.id) :=
+  In C prog_comps.
+Definition is_context_component C (prog_comps : list Component.id) :=
+  ~ (In C prog_comps).
 
-    | Program_Internal_Call:
-        forall mem C pc regs d d' C' P,
-          executing (Call C' P) C mem pc ->
-          C' <> C ->
-          call_exists Is C' P ->
-          call_permitted Is C C' P ->
-          is_program_component C' E ->
-          d' = (C,Some (pc+1)) :: d ->
-          let t := [ECall C P (Register.get Register.R_COM regs) C'] in
-          Is;E |-PLTT (PC (C,d,mem,regs,pc)) =>[t]
-                      (PC (C',d',mem,regs,EntryPoint.get C' P E))
+Reserved Notation "G |-PLTT s1 '=>[' t ']' s2" (at level 40).
 
-    | Program_Internal_Return:
-        forall mem C C' pc pc' d d' regs,
-          executing Return C mem pc ->
-          is_program_component C' E ->
-          d = (C',Some pc') :: d' ->
-          let t := [ERet C (Register.get Register.R_COM regs) C'] in
-          Is;E |-PLTT (PC (C,d,mem,regs,pc)) =>[t] (PC (C',d',mem,regs,pc'))
+Inductive step (G : global_env)
+  : partial_state -> trace -> partial_state -> Prop :=
+| Program_Epsilon:
+    forall C s ps mem mem' wmem wmem' cmem cmem' regs regs' pc pc',
+      M.MapsTo C cmem wmem ->
+      M.MapsTo C cmem' wmem' ->
+      let G' := LTT.mkGlobalEnv (get_interfaces G) (get_entrypoints G) in
+      LTT.step G' (C,s,wmem,regs,pc) E0 (C,s,wmem',regs',pc') ->
+      M.MapsTo C cmem mem ->
+      M.MapsTo C cmem' mem' ->
+      G |-PLTT (PC (C,ps,mem,regs,pc)) =>[E0] (PC (C,ps,mem',regs',pc'))
 
-    | Program_External_Call:
-        forall mem C pc regs d d' C' P,
-          executing (Call C' P) C mem pc ->
-          C' <> C ->
-          call_exists Is C' P ->
-          call_permitted Is C C' P ->
-          is_context_component C' E ->
-          d' = (C,Some (pc+1)) :: d ->
-          let t := [ECall C P (Register.get Register.R_COM regs) C'] in
-          Is;E |-PLTT (PC (C,d,mem,regs,pc)) =>[t] (CC (C',d',mem))
+| Program_Internal_Call:
+    forall mem C pc regs d d' C' P,
+      executing (Call C' P) C mem pc ->
+      C' <> C ->
+      call_is_public_and_exists (get_interfaces G) C' P ->
+      call_is_in_imports (get_interfaces G) C C' P ->
+      is_program_component C' (get_split G) ->
+      d' = (C,Some (pc+1)) :: d ->
+      let t := [ECall C P (Register.get Register.R_COM regs) C'] in
+      G |-PLTT (PC (C,d,mem,regs,pc)) =>[t]
+               (PC (C',d',mem,regs,EntryPoint.get C' P (get_entrypoints G)))
 
-    | Program_External_Return:
-        forall mem C C' pc d d' regs,
-          executing Return C mem pc ->
-          d = (C',None) :: d' ->
-          is_context_component C' E ->
-          let t := [ERet C (Register.get Register.R_COM regs) C'] in
-          Is;E |-PLTT (PC (C,d,mem,regs,pc)) =>[t] (CC (C',d',mem))
+| Program_Internal_Return:
+    forall mem C C' pc pc' d d' regs,
+      executing Return C mem pc ->
+      is_program_component C' (get_split G) ->
+      d = (C',Some pc') :: d' ->
+      let t := [ERet C (Register.get Register.R_COM regs) C'] in
+      G |-PLTT (PC (C,d,mem,regs,pc)) =>[t] (PC (C',d',mem,regs,pc'))
 
-    | Context_Internal_Call:
-        forall mem C d d' C' P call_arg,
-          C' <> C ->
-          call_exists Is C' P ->
-          call_permitted Is C C' P ->
-          is_context_component C' E ->
-          d' = (C,None) :: d ->
-          let t := [ECall C P call_arg C'] in
-          Is;E |-PLTT (CC (C,d,mem)) =>[t] (CC (C',d',mem))
+| Program_External_Call:
+    forall mem C pc regs d d' C' P,
+      executing (Call C' P) C mem pc ->
+      C' <> C ->
+      call_is_public_and_exists (get_interfaces G) C' P ->
+      call_is_in_imports (get_interfaces G) C C' P ->
+      is_context_component C' (get_split G) ->
+      d' = (C,Some (pc+1)) :: d ->
+      let t := [ECall C P (Register.get Register.R_COM regs) C'] in
+      G |-PLTT (PC (C,d,mem,regs,pc)) =>[t] (CC (C',d',mem))
 
-    | Context_Internal_Return:
-        forall mem C C' d d' return_val,
-          C' <> C ->
-          is_context_component C' E ->
-          d = (C',None) :: d' ->
-          let t := [ERet C return_val C'] in
-          Is;E |-PLTT (CC (C,d,mem)) =>[t] (CC (C',d',mem))
+| Program_External_Return:
+    forall mem C C' pc d d' regs,
+      executing Return C mem pc ->
+      d = (C',None) :: d' ->
+      is_context_component C' (get_split G) ->
+      let t := [ERet C (Register.get Register.R_COM regs) C'] in
+      G |-PLTT (PC (C,d,mem,regs,pc)) =>[t] (CC (C',d',mem))
 
-    | Context_External_Call:
-        forall mem C regs d d' C' P,
-          C' <> C ->
-          call_exists Is C' P ->
-          call_permitted Is C C' P ->
-          is_program_component C' E ->
-          d' = (C,None) :: d ->
-          let t := [ECall C P (Register.get Register.R_COM regs) C'] in
-          Is;E |-PLTT (CC (C,d,mem)) =>[t]
-                      (PC (C',d',mem,regs,EntryPoint.get C' P E))
+| Context_Internal_Call:
+    forall mem C d d' C' P call_arg,
+      C' <> C ->
+      call_is_public_and_exists (get_interfaces G) C' P ->
+      call_is_in_imports (get_interfaces G) C C' P ->
+      is_context_component C' (get_split G) ->
+      d' = (C,None) :: d ->
+      let t := [ECall C P call_arg C'] in
+      G |-PLTT (CC (C,d,mem)) =>[t] (CC (C',d',mem))
 
-    | Context_External_Return:
-        forall mem C C' pc' d d' regs,
-          d = (C',Some pc') :: d' ->
-          is_program_component C' E ->
-          let t := [ERet C (Register.get Register.R_COM regs) C'] in
-          Is;E |-PLTT (CC (C,d,mem)) =>[t] (PC (C',d',mem,regs,pc'))
+| Context_Internal_Return:
+    forall mem C C' d d' return_val,
+      C' <> C ->
+      is_context_component C' (get_split G) ->
+      d = (C',None) :: d' ->
+      let t := [ERet C return_val C'] in
+      G |-PLTT (CC (C,d,mem)) =>[t] (CC (C',d',mem))
 
-  where "Is ; E |-PLTT s1 '=>[' t ']' s2" := (step Is E s1 t s2).
+| Context_External_Call:
+    forall mem C regs d d' C' P,
+      C' <> C ->
+      call_is_public_and_exists (get_interfaces G) C' P ->
+      call_is_in_imports (get_interfaces G) C C' P ->
+      is_program_component C' (get_split G) ->
+      d' = (C,None) :: d ->
+      let t := [ECall C P (Register.get Register.R_COM regs) C'] in
+      G |-PLTT (CC (C,d,mem)) =>[t]
+               (PC (C',d',mem,regs,EntryPoint.get C' P (get_entrypoints G)))
+
+| Context_External_Return:
+    forall mem C C' pc' d d' regs,
+      d = (C',Some pc') :: d' ->
+      is_program_component C' (get_split G) ->
+      let t := [ERet C (Register.get Register.R_COM regs) C'] in
+      G |-PLTT (CC (C,d,mem)) =>[t] (PC (C',d',mem,regs,pc'))
+
+where "G |-PLTT s1 '=>[' t ']' s2" := (step G s1 t s2).
+
 End PLTT.
